---
layout: post
title:  "Vieta Root Jumping"
date:   2014-09-21 16:00:00
first-language: En
second-language: Pt
subdomain: pt
activate-lan: yes
categories: post
---

Hello guys, this post is about a nice number theory proof technique useful in math contest like [IMO][IMO], [IMC][IMC], etc. called the <b>Vieta Root Jumping</b>.
The Vieta jumping, which involve the common theme of a proof by infinite descent, by example thanks to Vieta jumping, we can get a <b>Markov tree</b>, which is generated by <b>Markov numbers</b>


<b>Markov number</b>
---

A Markov number is a positive integer $$x$$, $$y$$ or $$z$$ that is part of a solution to the Markov Diophantine Equation:
$$ x^{2} + y^{2} + z^{2} = 3xyz$$, so through  previous equation we get the sequence [$$ 1, 2, 5, 13, 29... $$][OEIS-A002559].

In particular one can normalize the triples so that $$ x \leqslant y \leqslant z$$. Then if $$(x, y, z)$$ is a Markov triple then by
Vieta jumping so is $$(x, y, 3xy-z)$$. Beautiful, isn't?

But how We got the $$(x, y, 3xy-z)$$? Well, we can do this through <b>Vieta's formulas</b>

<b>Vieta's formula</b>
---

Vieta's formulas are formulas that relate the coefficients of a polynomial to sums and products of its roots.
Any general polynomial of degree $$n$$

$$
P(x) = a_{n}x^{n} + a_{n-1}x^{n-1} + ... + a_{1}x + a_{0}
$$

(with the coefficients being real or complex numbers and $$a_{n} \neq 0$$) is known by the <b>Fundamental theorem of algebra</b> to have $$n$$ complex roots
$$x_{1}, x_{2}, ..., x_{n}$$. Vieta's formulas relate the polynomial's coefficients {$$a_{k}$$} to signed sums and products of its roots {$$x_{i}$$}
as follows:


$$
\left\{ \begin{array}{llll} 
x_{1} + x_{2} + ... + x_{n-1} + x_{n} = -\frac{a_{n-1}}{a_{n}} \\
(x_{1}x_{2} + x_{1}x_{3} + ... + x_{1}x_{n}) + (x_{2}x_{3} + x_{2}x_{4} + ... + x_{2}x_{n}) + ... + x_{n-1}x_{n} = \frac{a_{n-2}}{a_{n}} \\
\vdots \\
x_{1}x_{2} ...x_{n} = (-1)^{n}\frac{a_{0}}{a_{n}},
\end{array}\right.
$$

Equivalently stated the ($$n-k$$)th coefficient $$a_{n-k}$$ is related to a signed sum of all possible subproducts of roots, taken $$k$$-at-a-time:

$$
\sum_{1 \leq i_{i} < i_{2} < ... < i_{k} \leq n}{x_{i_{1}}x_{i_{2}} ...x_{i_{k}} = (-1)^{k}\frac{a_{n-k}}{a_{n}}}
$$

By example:

For the polynomial $$P(x) = ax^{3} + bx^{2} + cx + d$$, roots $$x_{1}, x_{2}, x_{3}$$ of the equation $$P(x) = 0$$ satisfy

$$x_{1} + x_{2} + x_{3} = -\frac{b}{a}, \ \ \ x_{1}x_{2} +x_{1}x_{3} + x_{2}x_{3} = \frac{c}{a}, \ \ \ x_{1}x_{2}x_{3} = -\frac{d}{a}$$

<b>Solving problems</b>
---

Already we have the basic definitions to prove some statements, so lets begin with the classical problem from IMO 1998:

<b>$$1.-$$ Let $$a$$ and $$b$$ be positive integers so that $$ab + 1$$ divides $$a^{2} + b^{2}$$. Prove that $$\frac{a^{2}+b^{2}}{ab+1}$$ is a perfect square.</b>

$$Solution$$

Let $$k = \frac{a^{2}+b^{2}}{ab+1}$$, we consider all the pairs $$(a, b)$$ non-negative which satisfy equation:

$$\frac{a^{2}+b^{2}}{ab+1} = k,$$ then  $$s =$$ {$$(a, b): a, b  \ \ \epsilon \ \ \mathbb{Z}^{+} \wedge \frac{a^{2}+b^2}{ab+1} = k$$}

There exists a pair $$(a, b)$$ where $$b=0$$, in this case we have:

$$
\frac{a^{2}+0}{a(0)+1} = k \\
a^{2} = k
$$

So, for this case our proof is complete. For prove this claim, we suppose that $$k$$ is not a perfect square and that $$(A, B \  \epsilon \ \  S)$$
is the pair that minimize $$a+b$$ over all pairs $$(a, b) \ \epsilon \ \ S$$. So, we assume that: $$A \geqslant B > 0$$, we have the equation:

$$
\frac{X^{2} + B^{2}}{XB + 1} = k,
$$

which is equivalent to:

$$
X^{2} - KBX + B^{2} - k = 0
$$

as a quadratic equation in $$X$$. We know that $$X_{1} = A$$ is one root of this equation, by Vieta's formula the another root of the equation is:

$$
X_{2} = \frac{(-1)^{2}(B^{2}-k)}{A} = \frac{B^{2}-k}{A}
$$

We realize that $$X_{2}$$ is an integer and $$X_{2}\neq0$$ since otherwise, $$k=B^{2}$$ would be a perfect square, contradicting our assumption.
Also, $$X_{2}$$ cannot be negative, for otherwise:

$$
X_{2}^{2} - kBX_{2} + B^{2} - k \geqslant X_{2}^{2} + k + B^{2} - k > 0,
$$

a contradiction, hence, $$X_{2} \geqslant 0$$ and thus $$(a, b) \  \epsilon \ \ S$$. However, because $$A \geqslant B$$, we have:

$$
X_{2} = \frac{B^{2}-k}{A} < A,
$$

So $$X_{2}+B < A+B$$, contradicting the minimality of $$A+B \ \$$ Q.E.D. 


<b>$$2.-$$ (IMO 2007) Let $$a, b$$ be positive integers. Show that if $$4ab-1$$ divides $$(4a^{2}-1)^{2}$$, then $$a=b$$</b>


$$
Solution
$$

Let $$k = \frac{(4a^{2}-1)^{2}}{(4ab-1)}$$, we consider the pair $$(a, b)$$ non-negative which satisfy this equation:

$$\frac{(4a^{2}-1)^{2}}{(4ab-1)} = k$$, Then $$s = $$ {$$(a,b): a, b \ \epsilon \ \ \mathbb{Z}^{+} \wedge \frac{(4a^{2}-1)^{2}}{(4ab-1)} = k$$},

There exists a pair $$(a, b)$$ where $$a=b$$, in this case we have:

<b>First case:</b>

$$
\frac{(4a^{2}-1)^{2}}{4a^{2}-1} = k 
$$

$$
(4a^{2}-1) = k
$$

Let's make $$2a=x$$, then $$(x^{2}-1) = k$$

<b>Second case:</b>

$$
\frac{(4b^{2}-1)^{2}}{4b^{2}-1} = k 
$$

$$
(4b^{2}-1) = k
$$

Let's make $$2b=y$$, then $$y^{2}-1 = k$$

Then,

$$
y^{2}-1 = x^{2}-1  \\

y = x
$$

Substituting 

$$
2a=2b
$$

$$
a=b
$$

So, for this case our proof is complete. For prove this claim, we suppose that $$a \neq b$$ and that $$(A, B) \ \epsilon \ \ s$$ is the pair
where $$a$$ and $$b$$ are never equals to all pairs $$(a, b) \ \ \epsilon \ s$$. So, we assume that $$(A > B > 0) \vee (0 < A < B)$$

Let's make  $$2A = X$$

$$
\frac{(X-1)^{2}}{XB - 1} = k
$$

Which is equivalent to say:

$$
X^{2} - 2X + 1 = XBK - K = 0 \\
x^{2}  - XBX - 2X + (1 + k) = 0
$$

As a quadratic equation in $$X$$. By Vieta's formula we know that $$X_{1}=2A$$ is one of roots of this equation, the another one is:

$$
X_{2} = \frac{-2X + (1+k)}{2A}
$$

We realize that $$X_{2}$$ is an integer and $$(A>B) \vee (B<A)$$, otherwise $$A$$ could be equal to $$B$$, contradicting our assumption. 
Also we note that for any $$k \ \epsilon \ \ \mathbb{Z}^{+}$$, Neither $$A>B$$ or $$B<A$$ is not strictly necessary. So,

$$
X_{2}^{2} - kBX_{2} - 2X_{2} + (1 + k) \geqslant X_{2}^{2} - X_{2} - 2X_{2} + (1 + k) \\

\\

\vee \\

\\

X_{2}^{2} - kBX_{2} - 2X_{2} + (1 + k) \leqslant X_{2}^{2} - X_{2} - 2X_{2} + (1 + k) \\
$$

A contradiction, hence $$a \neq b$$. So $$X_{2} + B \leqslant A + B$$, contradicting the statement of $$A \neq B$$. Q.E.D


[IMO]: http://imo-official.org/ 
[IMC]: http://www.imc-math.org.uk/
[OEIS-A002559]: https://oeis.org/A002559
